![image](https://github.com/user-attachments/assets/b5d291af-49bf-4950-9539-67eb48a8048d)

A, C
---

![image](https://github.com/user-attachments/assets/8fd2a116-15cf-426d-b2ac-9ad6eaaad71d)
To solve the problem, we need to analyze the function \( f(x) \) defined as follows:

$$
f(x) = 
\begin{cases} 
x^2 - |x| & \text{if } x < 0, \\
x^2 + |x| & \text{if } x \geq 0.
\end{cases}
$$

### Step 1: Simplify the Function
We can simplify the function based on the definition of the absolute value \( |x| \):

- For \( x < 0 \), \( |x| = -x \). Thus,
  $$
  f(x) = x^2 - |x| = x^2 - (-x) = x^2 + x.
  $$

- For \( x \geq 0 \), \( |x| = x \). Thus,
  $$
  f(x) = x^2 + |x| = x^2 + x.
  $$

So, the function can be rewritten as:
$$
f(x) = 
\begin{cases} 
x^2 + x & \text{if } x < 0, \\
x^2 + x & \text{if } x \geq 0.
\end{cases}
$$

This simplifies to:
$$ f(x) = x^2 + x \quad \text{for all } x \in \mathbb{R}. $$

### Step 2: Check Continuity at \( x = 0 \)
Since \( f(x) = x^2 + x \) is a polynomial function, it is continuous everywhere, including at \( x = 0 \). Therefore, \( f \) is continuous at \( x = 0 \).

### Step 3: Check Differentiability at \( x = 0 \)
To check differentiability at \( x = 0 \), we need to verify that the left-hand derivative (LHD) and the right-hand derivative (RHD) at \( x = 0 \) exist and are equal.

The derivative of \( f(x) = x^2 + x \) is:
$$
f'(x) = 2x + 1.
$$

- The left-hand derivative at \( x = 0 \) is:
  $$
  f'_-(0) = \lim_{h \to 0^-} \frac{f(0 + h) - f(0)}{h} = \lim_{h \to 0^-} \frac{(h^2 + h) - 0}{h} = \lim_{h \to 0^-} (h + 1) = 1.
  $$

- The right-hand derivative at \( x = 0 \) is:
  $$
  f'_+(0) = \lim_{h \to 0^+} \frac{f(0 + h) - f(0)}{h} = \lim_{h \to 0^+} \frac{(h^2 + h) - 0}{h} = \lim_{h \to 0^+} (h + 1) = 1.
  $$

Since \( f'_-(0) = f'_+(0) = 1 \), the function is differentiable at \( x = 0 \).

### Step 4: Check Continuity and Differentiability at \( x = 1 \)
Since \( f(x) = x^2 + x \) is a polynomial function, it is both continuous and differentiable everywhere, including at \( x = 1 \).

### Conclusion
From the analysis, we have:
1. \( f \) is not differentiable at \( x = 0 \): **False** (It is differentiable at \( x = 0 \)).
2. \( f \) is continuous at \( x = 0 \): **True**.
3. \( f \) is differentiable at \( x = 1 \): **True**.
4. \( f \) is not continuous at \( x = 1 \): **False** (It is continuous at \( x = 1 \)).

Thus, the correct options are:
$$
\boxed{f \text{ is continuous at } x = 0, \text{ and } f \text{ is differentiable at } x = 1.}
$$


---

### USER
![image](https://github.com/user-attachments/assets/2281eb89-921f-45fc-a10d-f290e133c940)


### ASSISTANT
To solve the problem, we need to analyze the function \( f(x) = x^2 + 2x - 8 \) and determine which of the given statements are true. Let's go through each statement step by step.

### Function Analysis
The given function is:
\[
f(x) = x^2 + 2x - 8
\]
This is a quadratic function, which represents a parabola. The general form of a quadratic function is:
\[
f(x) = ax^2 + bx + c
\]
Here, \( a = 1 \), \( b = 2 \), and \( c = -8 \).

### Statement 1: \( f \) is one-one on its domain.
A function is one-to-one if every horizontal line intersects the graph at most once. For a quadratic function \( f(x) = ax^2 + bx + c \), this is not generally true because the parabola is symmetric about its vertex, and thus it fails the horizontal line test unless the domain is restricted.

- The vertex of the parabola is the point where the function changes direction. For a quadratic function \( f(x) = ax^2 + bx + c \), the x-coordinate of the vertex is given by:
  \[
  x = -\frac{b}{2a}
  \]
  Substituting \( a = 1 \) and \( b = 2 \):
  \[
  x = -\frac{2}{2 \cdot 1} = -1
  \]
  So, the vertex is at \( x = -1 \). Since the parabola opens upwards (because \( a > 0 \)), the function is not one-to-one over its entire domain \( (-\infty, \infty) \).

**Conclusion for Statement 1:** False.

### Statement 2: \( f \) has an inverse on its domain.
A function has an inverse if and only if it is one-to-one. As we determined in Statement 1, \( f(x) \) is not one-to-one over its entire domain. Therefore, it does not have an inverse over its entire domain.

**Conclusion for Statement 2:** False.

### Statement 3: The vertex of this parabola is at \( (-1, -9) \).
We already calculated the x-coordinate of the vertex as \( x = -1 \). To find the y-coordinate of the vertex, we substitute \( x = -1 \) back into the function:
\[
f(-1) = (-1)^2 + 2(-1) - 8 = 1 - 2 - 8 = -9
\]
Thus, the vertex of the parabola is indeed at \( (-1, -9) \).

**Conclusion for Statement 3:** True.

### Statement 4: The y-intercept of the given parabola is \( -8 \).
The y-intercept of a function is the value of \( f(x) \) when \( x = 0 \). Substituting \( x = 0 \) into the function:
\[
f(0) = 0^2 + 2(0) - 8 = -8
\]
Thus, the y-intercept is \( -8 \).

**Conclusion for Statement 4:** True.

### Final Answer
The true statements are:
- Statement 3: The vertex of this parabola is at \( (-1, -9) \).
- Statement 4: The y-intercept of the given parabola is \( -8 \).

\[
\boxed{\text{The vertex of this parabola is at } (-1, -9), \text{ and the y-intercept of the given parabola is } -8.}
\]
